Refactor implementation of linkes lists

src/linear/aux/DoublyLinkedList.dfy
@@ -227,8 +227,7 @@ class DoublyLinkedList {
     ensures Model() == [x] + old(Model())
     ensures Repr() > old(Repr())
     ensures fresh(Repr() - old(Repr()))
-    // ensures old(head) != null ==> head != null
-    // ensures old(head) != null && old(head.next) == null ==> head.next == null
+    ensures spine == [head] + old(spine)
     ensures spine[1..] == old(spine)
   {
     var n := new DNode(null, x, head);
@@ -240,7 +239,7 @@ class DoublyLinkedList {
     assert head !in old(Repr());
   }
 
-  method Insert(mid: DNode, x: A) returns (node: DNode)
+  method Insert(mid: DNode, x: A)
     modifies this, Repr()
     requires Valid()
     requires mid in Repr()
@@ -257,18 +256,18 @@ class DoublyLinkedList {
       DistinctSpine();
       ModelRelationWithSpine();
     }
-    node := new DNode(mid, x, mid.next);
-    assert node.prev == mid;
-    assert node.prev == mid;
+    var n := new DNode(mid, x, mid.next);
+    assert n.prev == mid;
+    assert n.prev == mid;
     ghost var i :| 0 <= i < |spine| && spine[i] == mid;
     if mid.next != null {
       assert spine[i+1] == mid.next;
       assert mid.next in Repr();
-      mid.next.prev := node;
+      mid.next.prev := n;
     }
-    mid.next := node;
+    mid.next := n;
     { // GHOST
-      spine := spine[..i+1] + [node] + spine[i+1..];
+      spine := spine[..i+1] + [n] + spine[i+1..];
       ModelRelationWithSpine();
     }
   }
